\begin{lemma}\label{lem:hcp-display-mix}
  If $\seq[{ \piPar{\cpPlug{E}{P}}{Q} }]{ \Gamma }$, then
  $\tm{\piPar{\cpPlug{E}{P}}{Q}} \equiv \tm{\cpPlug{E}{\piPar{P}{Q}}}$. 
\end{lemma}
\begin{proof}
  By induction on the structure of the evaluation context $\tm{E}$.
  \begin{itemize}
  \item
    Case $\tm{\hole}$. By reflexivity.
  \item
    Case $\tm{\cpCut{x}{E}{R}}$.
    \begin{gather*}
      \begin{array}{lcl}
        \tm{\piPar{\cpCut{x}{\cpPlug{E}{P}}{R}}{Q}}     &\equiv &\text{by }\hcpEquivMixComm \\
        \tm{\piPar{Q}{\cpCut{x}{\cpPlug{E}{P}}{R}}}     &\equiv &\text{by }\hcpEquivMixCut2 \\
        \tm{\cpCut{x}{( \piPar{Q}{\cpPlug{E}{P}} )}{R}} &\equiv &\text{by }\cpEquivCutComm \\
        \tm{\cpCut{x}{( \piPar{\cpPlug{E}{P}}{Q} )}{R}} &\equiv &\text{by the induction hypothesis}\\
        \tm{\cpCut{x}{\cpPlug{E}{\piPar{P}{Q}}}{R}}
      \end{array}
    \end{gather*}
  \item
    Case $\tm{\cpCut{x}{R}{E}}$.
    \begin{gather*}
      \begin{array}{lcl}
        \tm{\piPar{\cpCut{x}{R}{\cpPlug{E}{P}}}{Q}}     &\equiv &\text{by }\hcpEquivMixComm \\
        \tm{\piPar{Q}{\cpCut{x}{\cpPlug{E}{P}}{R}}}     &\equiv &\text{by }\hcpEquivMixCut2 \\
        \tm{\cpCut{x}{( \piPar{Q}{\cpPlug{E}{P}} )}{R}} &\equiv &\text{by }\cpEquivCutComm \\
        \tm{\cpCut{x}{R}{( \piPar{Q}{\cpPlug{E}{P}} )}} &\equiv &\text{by the induction hypothesis} \\
        \tm{\cpCut{x}{R}{\cpPlug{E}{\piPar{P}{Q}}}}
      \end{array}
    \end{gather*}
  \item
    Case $\tm{\piPar{E}{R}}$.
    \begin{gather*}
      \begin{array}{lcl}
        \tm{\piPar{( \piPar{\cpPlug{E}{P}}{R} )}{Q}} &\equiv &\text{by }\hcpEquivMixComm \\
        \tm{\piPar{( \piPar{R}{\cpPlug{E}{P}} )}{Q}} &\equiv &\text{by }\hcpEquivMixAss2 \\
        \tm{\piPar{R}{( \piPar{\cpPlug{E}{P}}{Q} )}} &\equiv &\text{by }\hcpEquivMixComm \\
        \tm{\piPar{( \piPar{\cpPlug{E}{P}}{Q} )}{R}} &\equiv &\text{by the induction hypothesis} \\
        \tm{\piPar{\cpPlug{E}{\piPar{P}{Q}}}{R}}
      \end{array}
    \end{gather*}
  \item
    Case $\tm{\piPar{R}{E}}$.
    \begin{gather*}
      \begin{array}{lcl}
        \tm{\piPar{( \piPar{R}{\cpPlug{E}{P}} )}{Q}} &\equiv &\text{by }\hcpEquivMixAss2 \\
        \tm{\piPar{R}{( \piPar{\cpPlug{E}{P}}{Q} )}} &\equiv &\text{by the induction hypothesis} \\
        \tm{\piPar{R}{\cpPlug{E}{\piPar{P}{Q}}}}
      \end{array}
    \end{gather*}
  \end{itemize}
  The side conditions for the induction hypothesis can be inferred from
  \cref{thm:hcp-preservation-equiv}.
\end{proof}
