\begin{theorem}\label{thm:hcp2hccp-equiv}
  If $\tm{P}\equiv\tm{Q}$ in \hcp, then $\tm{\mtf{P}}\equiv\tm{\mtf{Q}}$ in \hccp.
\end{theorem}
\begin{proof}
  By induction on the structure of the derivation of $\tm{P}\equiv\tm{Q}$.
  \begin{itemize}
  \item
    Case \hcpEquivCutComm.
    \begin{gather*}
      \begin{array}{lcl}
        \tm{\piNew{x}{(\piPar{\mtf{P}}{\mtf{Q}})}}
        & \equiv & \text{by \hccpEquivMixComm}
        \\
        \tm{\piNew{x}{(\piPar{\mtf{Q}}{\mtf{P}})}}
      \end{array}
    \end{gather*}
  \item
    Case \hcpEquivCutAss1.
    \begin{gather*}
      \begin{array}{lcl}
        \tm{\piNew{x}{(\piPar{\mtf{P}}{\piNew{y}{(\piPar{\mtf{Q}}{\mtf{R}})}})}}
        & \equiv & \text{by \hccpEquivScopeExt2}
        \\
        \tm{\piNew{x}{\piNew{y}{(\piPar{\mtf{P}}{(\piPar{\mtf{Q}}{\mtf{R}})})}}}
        & \equiv & \text{by \hccpEquivNewComm}
        \\
        \tm{\piNew{y}{\piNew{x}{(\piPar{\mtf{P}}{(\piPar{\mtf{Q}}{\mtf{R}})})}}}
        & \equiv & \text{by \hccpEquivMixAss1}
        \\
        \tm{\piNew{y}{\piNew{x}{(\piPar{(\piPar{\mtf{P}}{\mtf{Q}})}{\mtf{R}})}}}
        & \equiv & \text{by \hccpEquivScopeExt1 and \hccpEquivMixComm}
        \\
        \tm{\piNew{y}{(\piPar{\piNew{x}{(\piPar{\mtf{P}}{\mtf{Q}})}}{\mtf{R}})}}
      \end{array}
    \end{gather*}
  \item
    Case \hcpEquivMixCut1.
    \begin{gather*}
      \begin{array}{lcl}
        \tm{\piNew{x}{(\piPar{(\piPar{P}{Q})}{R})}}
        & \equiv & \text{by \hccpEquivMixAss2}
        \\
        \tm{\piNew{x}{(\piPar{P}{(\piPar{Q}{R})})}}
        & \equiv & \text{by \hccpEquivScopeExt1}
        \\
        \tm{(\piPar{P}{\piNew{x}{(\piPar{Q}{R})}})}
      \end{array}
    \end{gather*}
  \end{itemize}
  The other cases are trivial.
\end{proof}
%%% Local Variables:
%%% TeX-master: "main"
%%% End:
